Test/Basic.lean
@@ -270,4 +270,3 @@ set_option trace.nunchaku true in
 example {n m : Nat} : n < m → n ≤ m := by
   nunchaku
   -/
-
